glue/riscv/falcon/bv32_falcon_lemmas.i.dfy
@@ -189,16 +189,6 @@ module bv32_falcon_lemmas refines generic_falcon_lemmas {
 
     const NORMSQ_BOUND := integers.BASE_31
 
-    function l2norm_squared(s1: seq<uint16>, s2: seq<uint16>, i: nat): nat
-        requires i <= N.full;
-        requires valid_nelems(s1);
-        requires valid_nelems(s2);
-    {
-        var ns1 := as_nelems(s1);
-        var ns2 := as_nelems(s2);
-        MQN.l2norm_squared(ns1, ns2, i)
-    }
-
     lemma accumulate_lemma(v16: uint16, sum: uint32, sum': uint32,
         over: uint32, over': uint32, gsum: nat)
         returns (gsum': nat)
@@ -271,36 +261,4 @@ module bv32_falcon_lemmas refines generic_falcon_lemmas {
             }
         }
     }
-
-    lemma falcon_lemma(
-        tt0: seq<uint16>, tt1: seq<uint16>, tt2: seq<uint16>,
-        s1: seq<uint16>, s2: seq<uint16>, h: seq<uint16>, c0: seq<uint16>,
-        result: uint32)
-
-    requires valid_elems(tt0);
-    requires valid_elems(tt1);
-    requires valid_elems(h);
-    requires denorm_inv(s2, tt0, 512);
-    requires as_elems(tt1) ==
-            poly_mod_product(as_elems(tt0), as_elems(h));
-    requires poly_sub_loop_inv(tt2, tt1, c0, 512);
-    requires norm_inv(s1, tt2, 512);
-    requires valid_nelems(s1);
-    requires valid_nelems(s2);
-    requires (result == 1) <==>
-        l2norm_squared(s1, s2, 512) < 0x29845d6;
-    ensures (result == 1) <==>
-        falcon_verify(as_elems(c0), as_nelems(s2), as_elems(h));
-    {
-        reveal valid_elems();
-        reveal norm_inv();
-
-        assert tt0 == MQN.denormalize_elems(as_nelems(s2));
-        assert tt1 == poly_mod_product(as_elems(tt0), as_elems(h));
-        assert tt2 == MQP.poly_sub(tt1, c0);
-        assert as_nelems(s1) == MQN.normalize_elems(tt2);
-        assert l2norm_squared(s1, s2, 512) == 
-            MQN.l2norm_squared(as_nelems(s1), as_nelems(s2), 512);
-    }
-
 }
